src/PlutusIR/Semantics/Static/normaliser_STLC/alpha/alpha.v
@@ -1277,3 +1277,5 @@ Proof.
     now apply not_in_app in Hfresh as [Hfresh1 Hfresh2].
   - constructor.
 Qed.
+
+
