src/PlutusIR/Semantics/Static/normaliser_STLC/gu_naive/step_gu.v
@@ -1,0 +1,382 @@
+From mathcomp Require Import ssreflect ssrbool eqtype ssrnat.
+From Coq Require Import ssrfun.
+Require Import Coq.Strings.String.
+Require Import Coq.Lists.List.
+From PlutusCert Require Import Util.List AutosubstSsr.
+Import ListNotations.
+Local Open Scope string_scope.
+Local Open Scope list_scope.
+Require Import Lia.
+Require Import Coq.Program.Basics.
+Require Import Coq.Arith.Arith.
+
+Set Implicit Arguments.
+Unset Strict Implicit.
+Unset Printing Implicit Defensive.
+From PlutusCert Require Import alpha_typing STLC_named STLC_named_typing ARS gu_naive.pre gu_naive.constructions.
+From PlutusCert Require Import alpha.alpha alpha_rename rename util alpha_ctx_sub freshness alpha_freshness.
+
+
+
+(* Examples
+λ x. x is GU_vars
+λ x. y is GU_vars
+λ x. λ y. x is GU_vars
+
+(λ x. x) y is GU_vars
+(λ x. x) x is not GU_vars (* free var is equal to a bound var*)
+(λ y. x) x is GU_vars (* all vars with the same name refer to the same term*)
+*)
+
+(* If a term has globally unique binders, then it has unique binders*)
+
+Inductive step_gu : term -> term -> Type :=
+| step_gu_intro s s' t : 
+    Alpha [] s s' ->
+    GU s' ->
+    step_naive s' t ->
+    step_gu s t.
+(*     
+    Alpha [] t' t ->
+    GU_vars t ->
+    step_gu s t. *)
+
+(** **** Many-Step Reduction 
+TODO: See if we can use the star from autosubst ARS again. (uses Prop instead of Set)
+*)
+Inductive red_gu_na : term -> term -> Type :=
+| red_gu_na_star s t t':
+     step_gu s t -> 
+     red_gu_na t t' ->
+     red_gu_na s t' 
+| red_gu_na_nil s :
+     red_gu_na s s.
+
+
+Lemma step_naive_preserves_alpha2 s t s' R:
+  GU s -> GU s' -> Alpha R s s' -> step_naive s t -> {t' & step_naive s' t' * Alpha R t t'}%type.
+Proof.
+  intros.
+  generalize dependent R.
+  generalize dependent s'.
+  induction H2; subst; intros.
+  - inversion H1; subst. inversion H7; subst.
+    
+    exists (sub y t2 s0).
+    split.
+    + constructor.
+    + eapply alpha_rename_binder_stronger; eauto with gu_nc_db.
+      constructor.
+  - inversion H1; subst.
+    specialize (IHstep_naive (gu_app_l H) s3 (gu_app_l H0) R H8) as [t' [Hstep_t' HR_t'] ].
+    exists (@tmapp B t' t2).
+    split; constructor; auto.
+  - inversion H1; subst.
+    specialize (IHstep_naive (gu_app_r H) t3 (gu_app_r H0) R H9) as [t' [Hstep_t' HR_t'] ].
+    exists (@tmapp B s2 t').
+    split; constructor; auto.
+  - inv H1.
+    specialize (IHstep_naive (gu_lam H) s3 (gu_lam H0) ((x, y)::R) H9) as [t' [Hstep_t' HR_t'] ].
+    exists (@tmlam B y A t').
+    split; constructor; auto.
+Qed.
+
+(* We need alpha here because global unique can create different terms depending on input:
+  global unique does not compose
+  suppose there is a free var in s2, then that must be renamed when doing step_gu (tmapp s1 s2)
+  while that is not the case in step_gu s1 t1 (there s2 does not need to be taken into account)
+  *)
+Lemma step_gu_app_l {B} s1 s2 t1 :
+  step_gu s1 t1 -> 
+  {t1' & Alpha [] t1 t1' * {s2' & Alpha [] s2 s2' * step_gu (@tmapp B s1 s2) (@tmapp B t1' s2')}%type }%type.
+Proof.
+  intros.
+
+  (* We cannot directly invert the (step_gu s1 t1), because we need something to be GU over s2 as well!*)
+  remember (to_GU (@tmapp B s1 s2)) as app.
+  remember Heqapp as Heqapp'. clear HeqHeqapp'.
+  apply to_GU_app_unfold in Heqapp.
+  destruct Heqapp as [s1' [s2' [ [Happ Ha_s1] Ha_s2] ] ].
+
+  inv H.
+
+  (* From step_naive s' t1, it then also follows that there must exist a t1' s.t. step_naive s1' t1'.*)
+  apply step_naive_preserves_alpha2 with (s' := s1') (R := nil) in H2 as [t1' [Hstep_s1' Ha_t1] ].
+  - exists t1'.
+    split; auto.
+    exists s2'.
+    split; auto.
+    apply step_gu_intro with (s' := (@tmapp B s1' s2')); auto.
+    + rewrite Heqapp'. apply to_GU__alpha.
+    + rewrite Heqapp'. apply to_GU__GU.
+    + constructor. auto.
+  - assumption.
+  - eapply gu_app_l. erewrite Heqapp'. apply to_GU__GU.
+  - eauto with α_eq_db.
+Qed.
+
+Lemma step_gu_na_lam_fold {B} x A s s' :
+  step_gu s s' -> {lams' & step_gu (@tmlam B x A s) lams' * Alpha [] lams' (@tmlam B x A s')}%type.
+Proof.
+  intros.
+  assert (Alpha [] (@tmlam B x A s) (to_GU (@tmlam B x A s)) ).
+  {
+    apply to_GU__alpha.
+  }
+  inversion H; subst.
+  rename s'0 into sgu.
+  inversion H0; subst.
+  assert (Alpha [(x, y)] sgu s2).
+  {
+    eapply @alpha_trans with (t := s) (ren := ((x, x)::nil)) (ren' := ((x, y)::nil)).
+    - constructor. constructor.
+    - apply alpha_extend_ids. constructor. constructor. eauto with α_eq_db.
+    - rewrite <- H10 in H0. inversion H0; subst. eauto.
+  } 
+  (* sgu and slam are both GU, so we can do step preserves 2*)
+  assert ({t' & step_naive s2 t' * Alpha [(x, y)] s' t'}%type).
+  {
+    eapply step_naive_preserves_alpha2.
+    - exact H2.
+    - assert (GU (to_GU (@tmlam B x A s))) by apply to_GU__GU.
+      rewrite <- H10 in H5. auto.
+      eapply gu_lam. eauto.
+    - eauto.
+    - auto.
+  }
+  destruct H5 as [t' [Hstep_t' Halpha_t'] ].
+  exists (@tmlam B y A t').
+  split.
+  - eapply step_gu_intro with (s' := tmlam y A s2); eauto.
+    + rewrite <- H10 in H0. eauto.
+    + assert (GU (to_GU (@tmlam B x A s))) by apply to_GU__GU.
+      rewrite <- H10 in H5. auto.
+    + apply step_abs. auto.
+  - eapply @alpha_sym. constructor. constructor. eauto.
+Qed.
+
+
+Lemma step_gu_preserves_alpha {s} {s'} {t} R :
+  Alpha R s t -> step_gu s s' -> {t' & prod (step_gu t t') (Alpha R s' t')}.
+Proof.
+  intros.
+  inversion H0; subst.
+  assert ({t' & step_naive (to_GU t) t' * Alpha R s' t'}%type).
+  {
+    eapply step_naive_preserves_alpha2; eauto.
+    + apply to_GU__GU.
+    + eapply @alpha_trans with (ren := ctx_id_left R) (ren' := R); eauto with α_eq_db.
+      * eapply id_left_trans.
+      * eapply alpha_extend_ids.
+        eapply ctx_id_left_is_id.
+        eapply @alpha_sym. constructor. exact H1.
+      * eapply @alpha_trans with (ren := R) (ren' := ctx_id_right R).
+        -- eapply id_right_trans.
+        -- eauto.
+        -- eapply alpha_extend_ids.
+           eapply ctx_id_right_is_id.
+           eapply to_GU__alpha.
+  }
+  destruct H4 as [t' [Hstep_t' HR_t'] ].
+  exists t'.
+  split.
+  - apply step_gu_intro with (s' := (to_GU t)); eauto.
+    + apply to_GU__alpha.
+    + apply to_GU__GU.
+  - auto.
+Qed.
+
+
+
+Lemma red_gu_naive_preserves_alpha {s} {s'} {t} R :
+  Alpha R s t -> red_gu_na s s' -> {t' & prod (red_gu_na t t') (Alpha R s' t')}.
+Proof.
+  intros.
+  generalize dependent R.
+  generalize dependent t.  
+  induction H0; intros.
+  - apply (step_gu_preserves_alpha H) in s0.
+    destruct s0 as [t'0 [Hstept'0 Ha_t'0] ].
+    specialize (IHred_gu_na t'0 R Ha_t'0).
+    destruct IHred_gu_na as [t'1 [Hred_t'1 Ha_t'1] ].
+    exists t'1.
+    split; auto.
+    apply red_gu_na_star with (t := t'0); auto.
+  - exists t.
+    split; auto.
+    constructor.
+Qed.
+
+(* step_gu/red_gu always freshens binders, hence we need to work up to alpha*)
+Lemma red_gu_na_lam_fold {B x A s s'} :
+  red_gu_na s s' -> {lams' & red_gu_na (@tmlam B x A s) lams' * Alpha [] lams' (@tmlam B x A s')}%type.
+Proof.
+  intros.
+  induction H.
+  - destruct IHred_gu_na as [lams' [Hred Halpha] ].
+
+    apply (@step_gu_na_lam_fold B x A) in s0.
+    destruct s0 as [lams'' [Hstep'' Halpha''] ].
+    assert ({lams''' & red_gu_na lams'' lams''' * Alpha [] lams' lams'''}%type).
+    {
+      apply @red_gu_naive_preserves_alpha with (t := lams'') (s := @tmlam B x A t); eauto with α_eq_db.
+    }
+    destruct H0 as [lams''' [Hred' Halpha'] ].
+    exists lams'''.
+    split.
+    + eapply red_gu_na_star.
+      * exact Hstep''.
+      * eauto.
+    + eauto with α_eq_db.
+  - exists (@tmlam B x A s).
+    split.
+    + apply red_gu_na_nil.
+    + apply alpha_refl. constructor.
+Qed.
+
+Lemma step_gu_na_appl_fold {B s1 s2 t1 }:
+  step_gu s1 s2 -> {app & step_gu (@tmapp B s1 t1) app * Alpha [] app (@tmapp B s2 t1)}%type.
+Proof.
+  intros Hstep_gu.
+  inversion Hstep_gu; subst.
+  assert (Hgu_a: nil ⊢ (@tmapp B s1 t1) ~ (to_GU (@tmapp B s1 t1))) by apply to_GU__alpha.
+  inversion Hgu_a; subst.
+
+  assert (Hstep_na': {s2' & step_naive s3 s2' * Alpha [] s2 s2'}%type).
+  {
+    eapply step_naive_preserves_alpha2; eauto.
+    - assert (Hgu_app: GU (to_GU (@tmapp B s1 t1))) by apply to_GU__GU.
+      rewrite <- H7 in Hgu_app.
+      eapply gu_app_l. eauto.
+    - assert (Alpha [] s1 (to_GU s1)) by apply to_GU__alpha.
+      eauto with α_eq_db.
+  }
+  destruct Hstep_na' as [s2' [Hstep_s2' Ha_s2'] ].
+  exists (@tmapp B s2' t2).
+  split.
+  - eapply step_gu_intro with (s' := @tmapp B s3 t2).
+    + rewrite H7. auto.
+    + rewrite H7. apply to_GU__GU.
+    + apply step_appL. auto.
+  - constructor; eauto with α_eq_db.
+Qed.
+
+Lemma step_gu_na_appr_fold {B s1 t1 t2 } : 
+  step_gu t1 t2 -> {app & step_gu (@tmapp B s1 t1) app * Alpha [] app (@tmapp B s1 t2)}%type.
+Proof.
+  intros Hstep_gu.
+  inversion Hstep_gu; subst.
+  assert (Hgu_a: nil ⊢ (@tmapp B s1 t1) ~ (to_GU (@tmapp B s1 t1))) by apply to_GU__alpha.
+  inversion Hgu_a; subst.
+
+  assert (Hstep_na': {t2' & step_naive t3 t2' * Alpha [] t2 t2'}%type).
+  {
+    eapply step_naive_preserves_alpha2; eauto.
+    - assert (Hgu_app: GU (to_GU (@tmapp B s1 t1))) by apply to_GU__GU.
+      rewrite <- H7 in Hgu_app.
+      eapply gu_app_r. eauto.
+    - assert (Alpha [] t1 (to_GU t1)) by apply to_GU__alpha.
+      eauto with α_eq_db.
+  }
+  destruct Hstep_na' as [t2' [Hstep_t2' Ha_t2'] ].
+  exists (@tmapp B s2 t2').
+  split.
+  - eapply step_gu_intro with (s' := @tmapp B s2 t3).
+    + rewrite H7. auto.
+    + rewrite H7. apply to_GU__GU.
+    + apply step_appR. auto.
+  - constructor; eauto with α_eq_db.
+Qed.
+
+Lemma red_gu_na_trans s t u :
+  red_gu_na s t -> red_gu_na t u -> red_gu_na s u.
+Proof.
+  intros.
+  generalize dependent u.
+  induction H; intros.
+  - generalize dependent s.
+    generalize dependent t.
+    induction H0; intros.
+    + eapply IHred_gu_na with (t := t0).
+      * eapply IHred_gu_na0.
+        eapply red_gu_na_star; eauto. constructor.
+      * intros.
+        eapply IHred_gu_na0.
+        eapply red_gu_na_star; eauto.
+      * auto.
+    + eapply red_gu_na_star; eauto.
+  - induction H0.
+    + eapply red_gu_na_star; eauto.
+    + constructor.
+Qed.
+
+Lemma red_gu_na_appl_fold {B s1 s2 t} :
+  red_gu_na s1 s2 -> {app & red_gu_na (@tmapp B s1 t) app * Alpha [] app (@tmapp B s2 t)}%type.
+Proof.
+  intros H0.
+  induction H0.
+    + destruct IHred_gu_na as [app [Hred Halpha] ].
+      eapply (@step_gu_na_appl_fold) with (s1 := s) (t1 := t) in s0.
+      destruct s0 as [app' [Hred' Halpha'] ].
+      assert ({app'' & red_gu_na app' app'' * Alpha [] app app''}%type).
+      {
+        eapply @red_gu_naive_preserves_alpha with (s := tmapp t0 t); eauto with α_eq_db.
+      }
+      destruct H as [app'' [Hred'' Halpha'' ] ].
+      exists app''.
+      split.
+      * eapply red_gu_na_star.
+        -- exact Hred'.
+        -- eauto.
+      * eauto with α_eq_db.
+    + exists (@tmapp B s t).
+      split.
+      * apply red_gu_na_nil.
+      * apply alpha_refl. constructor. 
+Qed.
+
+Lemma red_gu_na_appr_fold {B s1 t1 t2} :
+  red_gu_na t1 t2 -> {app & red_gu_na (@tmapp B s1 t1) app * Alpha [] app (@tmapp B s1 t2)}%type.
+Proof.
+  intros H0.
+  induction H0.
+    + destruct IHred_gu_na as [app [Hred Halpha] ].
+      eapply (@step_gu_na_appr_fold) with (s1 := s1) (t1 := s) (t2 := t) in s0.
+      destruct s0 as [app' [Hred' Halpha'] ].
+      assert ({app'' & red_gu_na app' app'' * Alpha [] app app''}%type).
+      {
+        eapply @red_gu_naive_preserves_alpha with (s := tmapp s1 t); eauto with α_eq_db.
+      }
+      destruct H as [app'' [Hred'' Halpha'' ] ].
+      exists app''.
+      split.
+      * eapply red_gu_na_star.
+        -- exact Hred'.
+        -- eauto.
+      * eauto with α_eq_db.
+    + exists (@tmapp B s1 s).
+      split.
+      * apply red_gu_na_nil.
+      * apply alpha_refl. constructor.
+Qed.
+
+Lemma red_gu_na_app_fold {B s1 s2 t1 t2} :
+  red_gu_na s1 s2 -> red_gu_na t1 t2 -> {app & red_gu_na (@tmapp B s1 t1) app * Alpha [] app (@tmapp B s2 t2)}%type.
+Proof.
+  intros.
+  eapply @red_gu_na_appl_fold with (t := t1) in H.
+  destruct H as [app [Hred Halpha] ].
+
+  eapply @red_gu_na_appr_fold with (s1 := s2) in H0.
+  destruct H0 as [app' [Hred' Halpha'] ].
+
+  assert ({app'' & red_gu_na app app'' * Alpha [] app' app''}%type).
+  {
+    eapply @red_gu_naive_preserves_alpha with (s := tmapp s2 t1); eauto with α_eq_db.
+  }
+  destruct H as [app'' [Hred'' Halpha'' ] ].
+  exists app''.
+  split.
+  - eapply red_gu_na_trans; eauto.
+  - eauto with α_eq_db.
+Qed.
